Semantic/Fsub/Substitution.lean
@@ -99,11 +99,11 @@ theorem TVar.weaken_subst_comm_liftMany {X : BVar (s1 ++ K) .tvar} {σ : Subst s
     | here => rfl
     | there X => rfl
   | cons k K ih =>
-    simp [Subst.liftMany, Rename.liftMany]
+    simp only [Subst.liftMany, Rename.liftMany]
     cases X with
     | here => rfl
     | there X =>
-      simp [Rename.lift_there_tvar_eq, Subst.lift_there_tvar_eq]
+      simp only [Rename.lift_there_tvar_eq, Subst.lift_there_tvar_eq]
       conv_rhs => rw [← ih]
       exact Ty.weaken_rename_comm
 
@@ -112,10 +112,10 @@ theorem Var.weaken_subst_comm_liftMany {x : Var (s1 ++ K)} {σ : Subst s1 s2} :
   (x.rename (Rename.succ.liftMany K)).subst (σ.lift (k:=k0).liftMany K) := by
   induction K with
   | nil =>
-    simp [Subst.liftMany, Rename.liftMany]
+    simp only [Subst.liftMany, Rename.liftMany]
     cases x <;> rfl
   | cons k K ih =>
-    simp [Subst.liftMany, Rename.liftMany]
+    simp only [Subst.liftMany, Rename.liftMany]
     cases x with
     | bound x =>
       cases x with
@@ -124,8 +124,8 @@ theorem Var.weaken_subst_comm_liftMany {x : Var (s1 ++ K)} {σ : Subst s1 s2} :
         conv => lhs; simp [Var.subst]
         conv => rhs; simp [Var.rename, Var.subst]
         have ih := ih (x:=.bound x)
-        simp [Var.subst, Var.rename] at ih
-        simp [Subst.lift_there_var_eq, Rename.lift_there_var_eq]
+        simp only [Var.subst, Var.rename] at ih
+        simp only [Subst.lift_there_var_eq, Rename.lift_there_var_eq]
         conv_rhs => rw [← ih]
         exact Var.weaken_rename_comm
     | free n => simp [Var.subst, Var.rename]
@@ -140,20 +140,24 @@ theorem Ty.weaken_subst_comm {T : Ty (s1 ++ K)} {σ : Subst s1 s2} :
   | .arrow T1 T2 =>
     have ih1 := Ty.weaken_subst_comm (T:=T1) (σ:=σ) (K:=K) (k0:=k0)
     have ih2 := Ty.weaken_subst_comm (T:=T2) (σ:=σ) (K:=K,x) (k0:=k0)
-    simp [Ty.subst, Ty.rename, ih1]
-    exact ih2
+    simp only [Ty.subst, Ty.rename, ih1]
+    simpa only [Subst.liftMany, Rename.liftMany] using
+      congrArg
+        (Ty.arrow ((T1.rename (Rename.succ.liftMany K)).subst (σ.lift.liftMany K)))
+        ih2
   | .poly T1 T2 =>
     have ih1 := Ty.weaken_subst_comm (T:=T1) (σ:=σ) (K:=K) (k0:=k0)
     have ih2 := Ty.weaken_subst_comm (T:=T2) (σ:=σ) (K:=K,X) (k0:=k0)
-    simp [Ty.subst, Ty.rename, ih1]
-    exact ih2
+    simp only [Ty.subst, Ty.rename, ih1]
+    simpa only [Subst.liftMany, Rename.liftMany] using
+      congrArg
+        (Ty.poly ((T1.rename (Rename.succ.liftMany K)).subst (σ.lift.liftMany K)))
+        ih2
 termination_by sizeOf T
 decreasing_by
   all_goals first
     | decreasing_tactic
     | (simp_wf; refine Nat.lt_add_of_pos_left ?_; omega)
-    | (simp_wf; refine Nat.lt_add_left _ ?_; exact Nat.succ_pos _)
-    | (simp_wf; omega)
 
 theorem Ty.weaken_subst_comm_base {T : Ty s1} {σ : Subst s1 s2} :
   (T.subst σ).rename (Rename.succ (k:=k)) = (T.rename Rename.succ).subst (σ.lift (k:=k)) :=
@@ -197,7 +201,7 @@ theorem Subst.comp_liftMany {σ1 : Subst s1 s2} {σ2 : Subst s2 s3} {K : Sig} :
   induction K with
   | nil => rfl
   | cons k K ih =>
-    simp [Subst.liftMany]
+    simp only [Subst.liftMany]
     conv_rhs => rw [← ih]
     exact Subst.comp_lift
 
@@ -222,11 +226,11 @@ theorem Ty.subst_comp {T : Ty s1} {σ1 : Subst s1 s2} {σ2 : Subst s2 s3} :
   | tvar x => rfl
   | singleton x => simp [Ty.subst, Var.subst_comp]
   | arrow T1 T2 ih1 ih2 =>
-    simp [Ty.subst, ih1, ih2]
+    simp only [Ty.subst, ih1, ih2]
     conv_rhs => rw [← Subst.comp_lift]
     rfl
   | poly T1 T2 ih1 ih2 =>
-    simp [Ty.subst, ih1, ih2]
+    simp only [Ty.subst, ih1, ih2]
     conv_rhs => rw [← Subst.comp_lift]
     rfl
 
@@ -239,17 +243,17 @@ theorem Exp.subst_comp {e : Exp s1} {σ1 : Subst s1 s2} {σ2 : Subst s2 s3} :
   induction e generalizing s2 s3 with
   | var x => simp [Exp.subst, Var.subst_comp]
   | abs T e ih_e =>
-    simp [Exp.subst, Ty.subst_comp, ih_e]
+    simp only [Exp.subst, Ty.subst_comp, ih_e]
     conv_rhs => rw [← Subst.comp_lift]
     rfl
   | tabs T e ih_e =>
-    simp [Exp.subst, Ty.subst_comp, ih_e]
+    simp only [Exp.subst, Ty.subst_comp, ih_e]
     conv_rhs => rw [← Subst.comp_lift]
     rfl
   | app x y => simp [Exp.subst, Var.subst_comp]
   | tapp x T => simp [Exp.subst, Var.subst_comp, Ty.subst_comp]
   | letin e1 e2 ih1 ih2 =>
-    simp [Exp.subst, ih1, ih2]
+    simp only [Exp.subst, ih1, ih2]
     conv_rhs => rw [← Subst.comp_lift]
     rfl
 
