Semantic/Fsub/Syntax.lean
@@ -56,12 +56,32 @@ def Var.rename_id {x : Var s} : x.rename (Rename.id) = x := by
   cases x <;> rfl
 
 def Ty.rename_id {T : Ty s} : T.rename (Rename.id) = T := by
-  induction T <;> (first | rfl | simp [Ty.rename, Var.rename_id, Rename.lift_id, *])
-    <;> first | rfl | assumption
+  induction T with
+  | top => rfl
+  | tvar x => rfl
+  | singleton x =>
+      simpa only [Ty.rename] using congrArg Ty.singleton (Var.rename_id (x:=x))
+  | arrow T1 T2 ih1 ih2 =>
+      simpa only [Ty.rename, Rename.lift_id, ih1] using congrArg (Ty.arrow T1) ih2
+  | poly T1 T2 ih1 ih2 =>
+      simpa only [Ty.rename, Rename.lift_id, ih1] using congrArg (Ty.poly T1) ih2
 
 def Exp.rename_id {e : Exp s} : e.rename (Rename.id) = e := by
-  induction e <;> (first | rfl | simp [Exp.rename, Ty.rename_id, Var.rename_id, Rename.lift_id, *])
-    <;> first | rfl | assumption
+  induction e with
+  | var x =>
+      simpa only [Exp.rename] using congrArg Exp.var (Var.rename_id (x:=x))
+  | abs T e ih =>
+      simpa only [Exp.rename, Ty.rename_id, Rename.lift_id] using congrArg (Exp.abs T) ih
+  | tabs T e ih =>
+      simpa only [Exp.rename, Ty.rename_id, Rename.lift_id] using congrArg (Exp.tabs T) ih
+  | app x y =>
+      rw [Exp.rename, Var.rename_id]
+      exact congrArg (Exp.app x) (Var.rename_id (x:=y))
+  | tapp x T =>
+      rw [Exp.rename, Var.rename_id]
+      exact congrArg (Exp.tapp x) (Ty.rename_id (T:=T))
+  | letin e1 e2 ih1 ih2 =>
+      simpa only [Exp.rename, Rename.lift_id, ih1] using congrArg (Exp.letin e1) ih2
 
 theorem Var.rename_comp {x : Var s1} {f : Rename s1 s2} {g : Rename s2 s3} :
     (x.rename f).rename g = x.rename (f.comp g) := by
@@ -69,15 +89,42 @@ theorem Var.rename_comp {x : Var s1} {f : Rename s1 s2} {g : Rename s2 s3} :
 
 theorem Ty.rename_comp {T : Ty s1} {f : Rename s1 s2} {g : Rename s2 s3} :
     (T.rename f).rename g = T.rename (f.comp g) := by
-  induction T generalizing s2 s3
-    <;> (first | rfl | simp [Ty.rename, Var.rename_comp, Rename.lift_comp, *])
-    <;> first | rfl | assumption
+  induction T generalizing s2 s3 with
+  | top => rfl
+  | tvar x => rfl
+  | singleton x =>
+      simpa only [Ty.rename] using congrArg Ty.singleton (Var.rename_comp (x:=x) (f:=f) (g:=g))
+  | arrow T1 T2 ih1 ih2 =>
+      simpa only [Ty.rename, Rename.lift_comp, ih1] using
+        congrArg (Ty.arrow (T1.rename (f.comp g))) (ih2 (f:=f.lift) (g:=g.lift))
+  | poly T1 T2 ih1 ih2 =>
+      simpa only [Ty.rename, Rename.lift_comp, ih1] using
+        congrArg (Ty.poly (T1.rename (f.comp g))) (ih2 (f:=f.lift) (g:=g.lift))
 
 theorem Exp.rename_comp {e : Exp s1} {f : Rename s1 s2} {g : Rename s2 s3} :
     (e.rename f).rename g = e.rename (f.comp g) := by
-  induction e generalizing s2 s3
-    <;> (first | rfl | simp [Exp.rename, Ty.rename_comp, Var.rename_comp, Rename.lift_comp, *])
-    <;> first | rfl | assumption
+  induction e generalizing s2 s3 with
+  | var x =>
+      simpa only [Exp.rename] using congrArg Exp.var (Var.rename_comp (x:=x) (f:=f) (g:=g))
+  | abs T e ih =>
+      simpa only [Exp.rename, Ty.rename_comp, Rename.lift_comp] using
+        congrArg (Exp.abs (T.rename (f.comp g))) (ih (f:=f.lift) (g:=g.lift))
+  | tabs T e ih =>
+      simpa only [Exp.rename, Ty.rename_comp, Rename.lift_comp] using
+        congrArg (Exp.tabs (T.rename (f.comp g))) (ih (f:=f.lift) (g:=g.lift))
+  | app x y =>
+      change
+        Exp.app ((x.rename f).rename g) ((y.rename f).rename g) =
+          Exp.app (x.rename (f.comp g)) (y.rename (f.comp g))
+      rw [Var.rename_comp, Var.rename_comp]
+  | tapp x T =>
+      change
+        Exp.tapp ((x.rename f).rename g) ((T.rename f).rename g) =
+          Exp.tapp (x.rename (f.comp g)) (T.rename (f.comp g))
+      rw [Var.rename_comp, Ty.rename_comp]
+  | letin e1 e2 ih1 ih2 =>
+      simpa only [Exp.rename, Rename.lift_comp, ih1] using
+        congrArg (Exp.letin (e1.rename (f.comp g))) (ih2 (f:=f.lift) (g:=g.lift))
 
 theorem Ty.weaken_rename_comm {T : Ty s1} {f : Rename s1 s2} :
     (T.rename Rename.succ).rename (f.lift (k:=k0)) = (T.rename f).rename (Rename.succ) := by
